[Civl] Generalizing PingPong (#533)
* generalizing sample to handle arbitrary number of PingPong pairs

* added documentation and renamed Permission to ChannelHandle

Test/civl/inductive-sequentialization/PingPong.bpl
@@ -1,16 +1,41 @@
 // RUN: %parallel-boogie "%s" > "%t"
 // RUN: %diff "%s.expect" "%t"
 
-type {:linear "pid"} Pid = int;
-var {:layer 0,3} ping_channel:[int]int; // Incoming channel of Ping
-var {:layer 0,3} pong_channel:[int]int; // Incoming channel of Pong
+// This example shows how to use a bidirectional shared channel to communicate between
+// two processes. The modeling of bidirectional channels is generic.
+// Its usage is specifically illustrated here on a PingPong example.
 
-const unique ping_id:int;
-const unique pong_id:int;
+// A bidirectional channel is a pair of ordinary channels with two ends---left and right.
+type {:datatype} ChannelPair;
+function {:constructor} ChannelPair(left: [int]int, right: [int]int): ChannelPair;
 
+// The id type for indexing into the pool of bidirectional channels.
+type ChannelId;
+
+// The following global variables models al instances of a bidirectional channel indexed
+// the ChannelId type. A single instance of PingPong will only use a single channel id.
+var {:layer 0,3} channel: [ChannelId]ChannelPair;
+
+// The id of a bidirectional channel can be split into two permissions---Left and Right.
+// Left permission is used to receive from the left channel and send to the right channel.
+// Right permission is used to receive from the right channel and send to the left channel.
+type {:linear "cid"} {:datatype} ChannelHandle;
+function {:constructor} Left(cid: ChannelId): ChannelHandle;
+function {:constructor} Right(cid: ChannelId): ChannelHandle;
+function {:inline} ChannelId(p: ChannelHandle) : ChannelId {
+  if is#Left(p) then cid#Left(p) else cid#Right(p)
+}
+
+function {:inline} {:linear "cid"} ChannelIdCollector(cid: ChannelId) : [ChannelHandle]bool {
+  MapConst(false)[Left(cid) := true][Right(cid) := true]
+}
+
+// This datatype declares the pending asyncs for Ping and Pong processes.
+// These two processes share a channel pair with Ping holding its left channel handle
+// and Pong holding its right channel handle.
 type {:pending_async}{:datatype} PA;
-function {:constructor} PING(x:int, pid:int) : PA;
-function {:constructor} PONG(x:int, pid:int) : PA;
+function {:constructor} PING(x: int, left: ChannelHandle): PA;
+function {:constructor} PONG(x: int, right: ChannelHandle): PA;
 
 function {:inline} NoPAs () : [PA]int
 { (lambda pa:PA :: 0) }
@@ -21,47 +46,37 @@ function {:inline} EmptyChannel () : [int]int
 ////////////////////////////////////////////////////////////////////////////////
 
 procedure {:atomic}{:layer 3}
-MAIN' ({:linear_in "pid"} ping_pid:int, {:linear_in "pid"} pong_pid:int)
+MAIN' ({:linear_in "cid"} cid: ChannelId)
 {
-  assert ping_pid == ping_id;
-  assert pong_pid == pong_id;
-  assert ping_channel == EmptyChannel();
-  assert pong_channel == EmptyChannel();
+  assert channel[cid] == ChannelPair(EmptyChannel(), EmptyChannel());
 }
 
 procedure {:IS_invariant}{:layer 2}
-INV ({:linear_in "pid"} ping_pid:int, {:linear_in "pid"} pong_pid:int)
-returns ({:pending_async "PING","PONG"} PAs:[PA]int, {:choice} choice:PA)
-modifies ping_channel, pong_channel;
+INV ({:linear_in "cid"} cid: ChannelId)
+returns ({:pending_async "PING","PONG"} PAs: [PA]int, {:choice} choice: PA)
+modifies channel;
 {
-   var {:pool "INV"} c: int;
+  var {:pool "INV"} c: int;
 
-  assert ping_pid == ping_id;
-  assert pong_pid == pong_id;
-  assert ping_channel == EmptyChannel();
-  assert pong_channel == EmptyChannel();
+  assert channel[cid] == ChannelPair(EmptyChannel(), EmptyChannel());
 
   assume
     {:add_to_pool "INV", c, c+1}
     0 < c;
   if (*) {
-    pong_channel := EmptyChannel()[c := 1];
-    ping_channel := EmptyChannel();
-    PAs := NoPAs()[PONG(c, pong_pid) := 1][PING(c, ping_pid) := 1];
-    choice := PONG(c, pong_pid);
+    channel[cid] := ChannelPair(EmptyChannel(), EmptyChannel()[c := 1]);
+    PAs := NoPAs()[PONG(c, Right(cid)) := 1][PING(c, Left(cid)) := 1];
+    choice := PONG(c, Right(cid));
   } else if (*) {
-    pong_channel := EmptyChannel()[0 := 1];
-    ping_channel := EmptyChannel();
-    PAs := NoPAs()[PONG(c, pong_pid) := 1];
-    choice := PONG(c, pong_pid);
+    channel[cid] := ChannelPair(EmptyChannel(), EmptyChannel()[0 := 1]);
+    PAs := NoPAs()[PONG(c, Right(cid)) := 1];
+    choice := PONG(c, Right(cid));
   } else if (*) {
-    ping_channel := EmptyChannel()[c := 1];
-    pong_channel := EmptyChannel();
-    PAs := NoPAs()[PONG(c+1, pong_pid) := 1][PING(c, ping_pid) := 1];
-    choice := PING(c, ping_pid);
+    channel[cid] := ChannelPair(EmptyChannel()[c := 1], EmptyChannel());
+    PAs := NoPAs()[PONG(c+1, Right(cid)) := 1][PING(c, Left(cid)) := 1];
+    choice := PING(c, Left(cid));
   } else {
-    ping_channel := EmptyChannel();
-    pong_channel := EmptyChannel();
+    channel[cid] := ChannelPair(EmptyChannel(), EmptyChannel());
     PAs := NoPAs();
   }
 }
@@ -69,165 +84,216 @@ modifies ping_channel, pong_channel;
 ////////////////////////////////////////////////////////////////////////////////
 
 procedure {:IS_abstraction}{:layer 2}
-PING' (x:int, {:linear_in "pid"} pid:int)
-returns ({:pending_async "PING"} PAs:[PA]int)
-modifies ping_channel, pong_channel;
+PING' (x: int, {:linear_in "cid"} left: ChannelHandle)
+returns ({:pending_async "PING"} PAs: [PA]int)
+modifies channel;
 {
-  assert (exists {:pool "INV"} m:int :: ping_channel[m] > 0) && (forall m:int :: pong_channel[m] == 0);
-  call PAs := PING(x, pid);
+  var cid: ChannelId;
+  var left_channel: [int]int;
+  var right_channel: [int]int;
+
+  cid := ChannelId(left);
+  left_channel := left#ChannelPair(channel[cid]);
+  right_channel := right#ChannelPair(channel[cid]);
+
+  assert (exists {:pool "INV"} m:int :: left_channel[m] > 0);
+  assert (forall m:int :: right_channel[m] == 0);
+  call PAs := PING(x, left);
 
 }
 
 procedure {:IS_abstraction}{:layer 2}
-PONG' (y:int, {:linear_in "pid"} pid:int)
-returns ({:pending_async "PONG"} PAs:[PA]int)
-modifies ping_channel, pong_channel;
+PONG' (y: int, {:linear_in "cid"} right: ChannelHandle)
+returns ({:pending_async "PONG"} PAs: [PA]int)
+modifies channel;
 {
-  assert (exists {:pool "INV"} m:int :: pong_channel[m] > 0) && (forall m:int :: ping_channel[m] == 0);
-  call PAs := PONG(y, pid);
+  var cid: ChannelId;
+  var left_channel: [int]int;
+  var right_channel: [int]int;
+
+  cid := ChannelId(right);
+  left_channel := left#ChannelPair(channel[cid]);
+  right_channel := right#ChannelPair(channel[cid]);
+
+  assert (exists {:pool "INV"} m:int :: right_channel[m] > 0);
+  assert (forall m:int :: left_channel[m] == 0);
+  call PAs := PONG(y, right);
 }
 
 ////////////////////////////////////////////////////////////////////////////////
 
 procedure {:atomic}{:layer 2}
 {:IS "MAIN'","INV"}{:elim "PING","PING'"}{:elim "PONG","PONG'"}
-MAIN ({:linear_in "pid"} ping_pid:int, {:linear_in "pid"} pong_pid:int)
-returns ({:pending_async "PING","PONG"} PAs:[PA]int)
-modifies pong_channel;
+MAIN ({:linear_in "cid"} cid: ChannelId)
+returns ({:pending_async "PING","PONG"} PAs: [PA]int)
+modifies channel;
 {
-  assert ping_pid == ping_id;
-  assert pong_pid == pong_id;
-  assert ping_channel == EmptyChannel();
-  assert pong_channel == EmptyChannel();
-  pong_channel[1] := pong_channel[1] + 1;
-  PAs := NoPAs()[PING(1, ping_pid) := 1][PONG(1, pong_pid) := 1];
+  assert channel[cid] == ChannelPair(EmptyChannel(), EmptyChannel());
+  channel[cid] := ChannelPair(EmptyChannel(), EmptyChannel()[1 := 1]);
+  PAs := NoPAs()[PING(1, Left(cid)) := 1][PONG(1, Right(cid)) := 1];
 }
 
 procedure {:atomic}{:layer 2}
-PING (x:int, {:linear_in "pid"} pid:int)
-returns ({:pending_async "PING"} PAs:[PA]int)
-modifies ping_channel, pong_channel;
+PING (x: int, {:linear_in "cid"} left: ChannelHandle)
+returns ({:pending_async "PING"} PAs: [PA]int)
+modifies channel;
 {
+  var cid: ChannelId;
+  var left_channel: [int]int;
+  var right_channel: [int]int;
+
+  cid := ChannelId(left);
+  left_channel := left#ChannelPair(channel[cid]);
+  right_channel := right#ChannelPair(channel[cid]);
+
   assert x > 0;
-  assert pid == ping_id;
-  assert (forall m:int :: ping_channel[m] > 0 ==> m == x); // assertion to discharge
+  assert is#Left(left);
+  assert (forall m:int :: left_channel[m] > 0 ==> m == x); // assertion to discharge
 
-  assume ping_channel[x] > 0;
-  ping_channel[x] := ping_channel[x] - 1;
+  assume left_channel[x] > 0;
+  left_channel[x] := left_channel[x] - 1;
 
   if (*)
   {
-    pong_channel[x+1] := pong_channel[x+1] + 1;
-    PAs := NoPAs()[PING(x+1, pid) := 1];
+    right_channel[x+1] := right_channel[x+1] + 1;
+    PAs := NoPAs()[PING(x+1, left) := 1];
   }
   else
   {
-    pong_channel[0] := pong_channel[0] + 1;
+    right_channel[0] := right_channel[0] + 1;
     PAs := NoPAs();
   }
+  channel[cid] := ChannelPair(left_channel, right_channel);
 }
 
 procedure {:atomic}{:layer 2}
-PONG (y:int, {:linear_in "pid"} pid:int)
-returns ({:pending_async "PONG"} PAs:[PA]int)
-modifies ping_channel, pong_channel;
+PONG (y: int, {:linear_in "cid"} right: ChannelHandle)
+returns ({:pending_async "PONG"} PAs: [PA]int)
+modifies channel;
 {
+  var cid: ChannelId;
+  var left_channel: [int]int;
+  var right_channel: [int]int;
+
+  cid := ChannelId(right);
+  left_channel := left#ChannelPair(channel[cid]);
+  right_channel := right#ChannelPair(channel[cid]);
+
   assert y > 0;
-  assert pid == pong_id;
-  assert (forall m:int :: pong_channel[m] > 0 ==> m == y || m == 0); // assertion to discharge
+  assert is#Right(right);
+  assert (forall m:int :: right_channel[m] > 0 ==> m == y || m == 0); // assertion to discharge
 
   if (*)
   {
-    assume pong_channel[y] > 0;
-    pong_channel[y] := pong_channel[y] - 1;
-    ping_channel[y] := ping_channel[y] + 1;
-    PAs := NoPAs()[PONG(y+1, pid) := 1];
+    assume right_channel[y] > 0;
+    right_channel[y] := right_channel[y] - 1;
+    left_channel[y] := left_channel[y] + 1;
+    PAs := NoPAs()[PONG(y+1, right) := 1];
   }
   else
   {
-    assume pong_channel[0] > 0;
-    pong_channel[0] := pong_channel[0] - 1;
+    assume right_channel[0] > 0;
+    right_channel[0] := right_channel[0] - 1;
     PAs := NoPAs();
   }
+  channel[cid] := ChannelPair(left_channel, right_channel);
 }
 
 ////////////////////////////////////////////////////////////////////////////////
 
 procedure {:yields}{:layer 1}{:refines "MAIN"}
-main ({:linear_in "pid"} ping_pid:int, {:linear_in "pid"} pong_pid:int)
+main ({:linear_in "cid"} cid: ChannelId)
 {
-  call send_pong_channel(1);
-  async call ping(1, ping_pid);
-  async call pong(1, pong_pid);
+  var {:linear "cid"} left: ChannelHandle;
+  var {:linear "cid"} right: ChannelHandle;
+
+  call left, right := split(cid);
+  call send(left, 1);
+  async call ping(1, left);
+  async call pong(1, right);
 }
 
 procedure {:yields}{:layer 1}{:refines "PING"}
-ping (x:int, {:linear_in "pid"} pid:int)
+ping (x: int, {:linear_in "cid"} left: ChannelHandle)
 {
-  var x':int;
+  var x': int;
 
-  call x' := receive_ping_channel();
-  call assert_eq(x', x); // low-level assertion to discharge
+  call x' := receive(left);
+  assert {:layer 1} x' == x; // low-level assertion to discharge
   if (*)
   {
-    call send_pong_channel(x'+1);
-    async call ping(x'+1, pid);
+    call send(left, x'+1);
+    async call ping(x'+1, left);
   }
   else
   {
-    call send_pong_channel(0);
+    call send(left, 0);
   }
 }
 
 procedure {:yields}{:layer 1}{:refines "PONG"}
-pong (y:int, {:linear_in "pid"} pid:int)
+pong (y: int, {:linear_in "cid"} right: ChannelHandle)
 {
-  var y':int;
+  var y': int;
 
-  call y' := receive_pong_channel();
+  call y' := receive(right);
   if (y' != 0)
   {
-    call assert_eq(y', y); // low-level assertion to discharge
-    call send_ping_channel(y');
-    async call pong(y'+1, pid);
+    assert {:layer 1} y' == y; // low-level assertion to discharge
+    call send(right, y');
+    async call pong(y'+1, right);
   }
 }
 
 ////////////////////////////////////////////////////////////////////////////////
+// Bidirectional channels
 
-procedure {:left}{:layer 1} SEND_PING_CHANNEL (m:int)
-modifies ping_channel;
+procedure {:right}{:layer 1} RECEIVE (permission: ChannelHandle) returns (m: int)
+modifies channel;
 {
-  ping_channel[m] := ping_channel[m] + 1;
+  var cid: ChannelId;
+  var left_channel: [int]int;
+  var right_channel: [int]int;
+
+  cid := ChannelId(permission);
+  left_channel := left#ChannelPair(channel[cid]);
+  right_channel := right#ChannelPair(channel[cid]);
+  if (is#Left(permission)) {
+    assume left_channel[m] > 0;
+    left_channel[m] := left_channel[m] - 1;
+  } else {
+    assume right_channel[m] > 0;
+    right_channel[m] := right_channel[m] - 1;
+  }
+  channel[cid] := ChannelPair(left_channel, right_channel);
 }
 
-procedure {:left}{:layer 1} SEND_PONG_CHANNEL (m:int)
-modifies pong_channel;
+procedure {:left}{:layer 1} SEND (permission: ChannelHandle, m: int)
+modifies channel;
 {
-  pong_channel[m] := pong_channel[m] + 1;
+  var cid: ChannelId;
+  var left_channel: [int]int;
+  var right_channel: [int]int;
+
+  cid := ChannelId(permission);
+  left_channel := left#ChannelPair(channel[cid]);
+  right_channel := right#ChannelPair(channel[cid]);
+  if (is#Left(permission)) {
+    right_channel[m] := right_channel[m] + 1;
+  } else {
+    left_channel[m] := left_channel[m] + 1;
+  }
+  channel[cid] := ChannelPair(left_channel, right_channel);
 }
 
-procedure {:right}{:layer 1} RECEIVE_PING_CHANNEL () returns (m:int)
-modifies ping_channel;
+procedure {:both}{:layer 1} SPLIT({:linear_in "cid"} cid: ChannelId)
+  returns ({:linear "cid"} left: ChannelHandle, {:linear "cid"} right: ChannelHandle)
 {
-  assume ping_channel[m] > 0;
-  ping_channel[m] := ping_channel[m] - 1;
+  left := Left(cid);
+  right := Right(cid);
 }
 
-procedure {:right}{:layer 1} RECEIVE_PONG_CHANNEL () returns (m:int)
-modifies pong_channel;
-{
-  assume pong_channel[m] > 0;
-  pong_channel[m] := pong_channel[m] - 1;
-}
-
-procedure {:both}{:layer 1} ASSERT_EQ (a:int, b:int)
-{
-  assert a == b;
-}
-
-procedure {:yields}{:layer 0}{:refines "SEND_PING_CHANNEL"} send_ping_channel (m:int);
-procedure {:yields}{:layer 0}{:refines "SEND_PONG_CHANNEL"} send_pong_channel (m:int);
-procedure {:yields}{:layer 0}{:refines "RECEIVE_PING_CHANNEL"} receive_ping_channel () returns (m:int);
-procedure {:yields}{:layer 0}{:refines "RECEIVE_PONG_CHANNEL"} receive_pong_channel () returns (m:int);
-procedure {:yields}{:layer 0}{:refines "ASSERT_EQ"} assert_eq (a:int, b:int);
+procedure {:yields}{:layer 0}{:refines "RECEIVE"} receive (permission: ChannelHandle) returns (m: int);
+procedure {:yields}{:layer 0}{:refines "SEND"} send (permission: ChannelHandle, m: int);
+procedure {:yields}{:layer 0}{:refines "SPLIT"} split({:linear_in "cid"} cid: ChannelId)
+  returns ({:linear "cid"} left: ChannelHandle, {:linear "cid"} right: ChannelHandle);
